build skeleton of decision procedure

theories/IterativeEquations.v
@@ -1,9 +1,11 @@
 Require Import CSL.IterativeContract.
 Require Import Setoid.
 Require Import Init.Tauto btauto.Btauto.
-Require Import Bool.Bool.
+Require Import Bool.Bool  Bool.Sumbool.
 Require Import Lists.List.
 Import ListNotations.
+Require Import Bool.Bool.
+From Equations Require Import Equations.
 (*******************************************************************************************************)
 Set Implicit Arguments.
 
@@ -128,7 +130,7 @@ Inductive c_eq_aci : Contract -> Contract -> Prop :=
     | cc_trans c0 c1 c2 (H1 : c0 =ACI= c1) (H2 : c1 =ACI= c2) : c0 =ACI= c2 (*transitivity*)
     | cc_ctx_plus c0 c0' c1 c1' (H1 : c0 =ACI= c0') (H2 : c1 =ACI= c1') : c0 _+_ c1 =ACI= c0' _+_ c1' (*ctx rules*)
     | cc_ctx_seq c0 c0' c1 c1' (H1 : c0 =ACI= c0') (H2 : c1 =ACI= c1') : c0 _;_ c1 =ACI= c0' _;_ c1'
-    where "c0 =ACI= c1" := (c_eq_aci c0 c1).
+    where "c0 =ACI= c1" := (c_eq_aci c0 c1). (*skip last three rules*)
 Hint Constructors c_eq_aci : core.
 
 Lemma c_eq_aci_nu : forall c0 c1, c0 =ACI= c1 -> nu c0 = nu c1.
@@ -170,7 +172,7 @@ intros. inversion H0.
 - apply H1.
 Qed.
 
-(*Co-recursive call only needed for showing -> *)
+
 Lemma c_eq_is_bisimilarity : bisimilarity c_eq.
 Proof. 
 split; generalize dependent c1; generalize dependent c0.
@@ -194,3 +196,178 @@ Proof.
 intros. pose proof c_eq_is_bisimilarity. pose proof matches_eq_is_bisimilarity.
 unfold bisimilarity in *. rewrite H0. now rewrite <- H1.
 Qed.
+
+(**********Decision procedure ******)
+
+Fixpoint trace_derive (c: Contract) (s : Trace) :=
+match s with
+| [] => c
+| e::s' => trace_derive (c/e) s'
+end.
+
+Lemma finitely_many_derivatives : forall c, exists (l : list Contract), (forall s, In (trace_derive c s) l).
+Proof. Admitted.
+
+Definition is_finite_bisimulation (l : list (Contract * Contract)) := 
+ forall c0 c1, In (c0,c1) l -> nu c0 = nu c1 /\ 
+                     forall (e : EventType), In (c0/e, c1/e) l.
+
+(*Decision procedure: 
+  to decide c0 = c1,
+  - compute list l, satisfying is_finite_bisimulation with respect to c0 and c1
+  - test (c0,c1) is present in the list
+ *)
+
+(*Showing bisimularity reduces to building a finite bisimulation list
+  and testing for membership*)
+Lemma in_finite_bisimulation_i_Bisimilarity : 
+ forall (l : list (Contract*Contract)) (c0 c1 : Contract), 
+ is_finite_bisimulation l -> In (c0,c1) l -> Bisimilarity c0 c1.
+Proof.
+cofix H.
+intros. constructor.
+- intro. apply H with l; auto. apply H0 in H1 as [_ H2];auto.
+- apply H0 in H1 as [H2 _];auto.
+Qed.
+
+Definition alphabet := [Notify;Transfer].
+Global Opaque alphabet.
+Definition direct_derivatives (c : Contract) : list Contract := map (fun e => c/e) alphabet.
+Check fold_left.
+Check filter.
+
+Section member.
+  Variable A : Set.
+  Hypothesis equals : A -> A -> bool.
+  
+  Fixpoint member (c : A) (l : list A) :=
+  match l with
+  | [] => false
+  | a::l' => equals a c || member c l' 
+  end.
+End member.
+
+Definition inclb (l0 l1 : list Contract) :bool := 
+ forallb (fun c0 => existsb (fun c1 => if eq_contract_dec c0 c1 then true else false) l1) l0.
+
+Lemma inclb_iff : forall (l0 l1 : list Contract), inclb l0 l1 = true <-> incl l0 l1.
+Proof. unfold inclb. unfold incl. split. 
+- intros. rewrite forallb_forall in H. apply H in H0. rewrite existsb_exists in H0. destruct H0 as [x [P0 P1]].
+destruct (eq_contract_dec a x).
+  * subst. assumption.
+  * discriminate.
+- intros. rewrite forallb_forall. intros. apply H in H0. rewrite existsb_exists. exists x. split.
+  * assumption.
+  * destruct (eq_contract_dec x x).
+    ** reflexivity.
+    ** contradiction. 
+Qed.
+
+
+Lemma incl_reflect : forall (l0 l1 : list Contract), reflect (incl l0 l1) (inclb l0 l1).
+Proof. 
+intros. destruct (inclb l0 l1) eqn:Heqn.
+- constructor. rewrite inclb_iff in Heqn. assumption.
+- constructor. intro H. rewrite <- inclb_iff in H. rewrite Heqn in H. discriminate.
+Qed.
+
+Fixpoint flatten_contract (c : Contract) : list Contract :=
+match c with
+| c0 _+_ c1 => (flatten_contract c0) ++ (flatten_contract c1)
+| _ => [c]
+end.
+
+Definition aci_eq (c0 c1 : Contract) : bool :=
+ let c0_l := flatten_contract c0 in
+ let c1_l := flatten_contract c1 in
+ (inclb c0_l c1_l) && (inclb c1_l c0_l) .
+
+Definition aci_p_eq (p0 p1: (Contract * Contract)) : bool :=
+ let (c0,c0') := p0 in
+ let (c1,c1') := p1 in
+ aci_eq c0 c1 && aci_eq c0' c1'.
+
+
+Fixpoint approx (A : Type) (n: nat) (f: A -> A) (arg: A) : A :=
+match n with
+| 0 => arg
+| S n' => approx n' f (f arg)
+end.
+
+Definition direct_p_derivatives (p : Contract * Contract) : list (Contract * Contract) := 
+ map (fun e => ((fst p) / e,(snd p) / e)) alphabet.
+
+Definition p_derivative_closure_once (l_pair : (list (Contract*Contract)) * (list (Contract * Contract))) :=
+ let (internal_nodes,leafs) := l_pair in
+ let internal_nodes' := internal_nodes++leafs in
+ let leaf_children := flat_map direct_p_derivatives leafs
+ in (internal_nodes',filter (fun c => negb (member aci_p_eq c internal_nodes')) leaf_children).
+
+Definition approx_p_derivative_closure (n : nat) (p : (Contract * Contract)) :=
+ approx n p_derivative_closure_once ([],[p]).
+
+Lemma p_derivative_closure_convergence : forall (c0 c1 : Contract), exists (n:nat),
+ approx_p_derivative_closure n (c0,c1) =  approx_p_derivative_closure (n+1) (c0,c1). 
+Proof. Admitted.
+
+Definition p_derivative_relation (arg_rec arg_inp : list (Contract*Contract) * list (Contract*Contract)) :=
+  p_derivative_closure_once arg_inp <> arg_inp /\  (*Not converged*)
+  p_derivative_closure_once arg_inp = arg_rec. (*is preceeding element*)
+
+Lemma well_founded_p_derivative_relation: well_founded p_derivative_relation.
+Proof. Admitted.
+
+Instance wf_p_derivative_relation : WellFounded p_derivative_relation := well_founded_p_derivative_relation.
+
+Lemma nil_i_convergence : forall (internal_nodes : list (Contract*Contract)),
+   p_derivative_closure_once (internal_nodes,[]) = (internal_nodes,[]).
+Proof. 
+intros. simpl. now rewrite <- app_nil_end.
+Qed.
+
+Lemma list_not_eq : forall (A:Type) (l0 l1 : list A) (p : A), l0++p::l1 = l0 -> False.
+Proof.
+intro. induction l0;intros.
+- discriminate.
+- inversion H. eauto. 
+Qed.
+
+
+Lemma cons_i_not_convergence : forall (p : Contract*Contract)(internal_nodes leafs : list (Contract*Contract)),
+   p_derivative_closure_once (internal_nodes,p::leafs) <> (internal_nodes,p::leafs).
+Proof.
+intros. simpl. intro H. injection H. intros.
+eauto using list_not_eq.
+Qed.
+
+Equations p_derivative_closure (internal_nodes_leafs : list (Contract*Contract) * list (Contract*Contract)) : list (Contract*Contract) by  wf internal_nodes_leafs p_derivative_relation :=
+p_derivative_closure (internal_nodes, []) := internal_nodes;
+p_derivative_closure (internal_nodes, leafs) := p_derivative_closure (p_derivative_closure_once (internal_nodes, leafs)).
+Next Obligation.
+unfold p_derivative_relation. split.
+- apply cons_i_not_convergence.
+- auto.
+Qed.
+Global Transparent p_derivative_closure.
+
+Definition derivative_closure (c0 c1 : Contract) := p_derivative_closure ([],[(c0,c1)]).
+Lemma in_derivative_closure : forall (c0 c1 : Contract), In (c0,c1) (derivative_closure c0 c1).
+Proof. Admitted.
+
+Definition decide_contract_equivalence (c0 c1 : Contract) := 
+ forallb (fun (p : Contract * Contract) => eqb (nu (fst p)) (nu (snd p)) ) (derivative_closure c0 c1).
+
+(*Forall Bisimilar c0 c1, there exists a finite_bisimulation list
+  ie, all contract equivalences can be decided by finding this list *)
+Lemma Bisimilarity_i_in_finite_bisimulation : 
+ forall (c0 c1 : Contract), Bisimilarity c0 c1 -> 
+   exists l, is_finite_bisimulation l /\ In (c0,c1) l.
+Proof. Admitted.
+
+Lemma Bisimilarity_reflected : forall (c0 c1 : Contract), reflect (Bisimilarity c0 c1) (decide_contract_equivalence c0 c1).
+Proof. Admitted.
+
+
+
+
+
